add fork primitive to Hazel and track forked off threads in EWP

theories/language/iris_language.v
@@ -23,9 +23,7 @@ From language Require Import syntax semantics neutral_contexts.
    relation that fits the format formalized by Iris. *)
 Definition prim_step' e1 σ1 (obs : list unit) e2 σ2 (efs : list expr) :=
   match obs with _ :: _ => False | [] =>
-    match efs with _ :: _ => False | [] =>
-      prim_step e1 σ1 e2 σ2
-    end
+      prim_step e1 σ1 e2 σ2 efs
   end.
 
 (* [eff_lang] satisfies the record type [LanguageMixin]. *)
@@ -34,7 +32,7 @@ Proof.
   split; apply _ || eauto using to_of_val, of_to_val.
   unfold prim_step'.
   intros e σ obs e' σ' efs.
-  case obs; [|done]; case efs; [|done].
+  case obs; [|done].
   induction 1 as [K e1' e2' -> ? ?].
   case K as [|f K].
   - revert H0. apply val_head_stuck.
@@ -55,7 +53,7 @@ Lemma reducible_fill_frame_eff f `{NeutralFrame f} m v k σ :
   reducible (fill_frame f (Eff m v k)) σ.
 Proof.
   unfold reducible. simpl. exists [], (Eff m v (f :: k)), σ, [].
-  apply (Ectx_prim_step _ _ _ _ [] (fill_frame f (Eff m v k))
+  apply (Ectx_prim_step _ _ _ _ _ [] (fill_frame f (Eff m v k))
                                         (Eff m v (f :: k))); eauto.
   by apply neutral_frame.
 Qed.
@@ -64,9 +62,9 @@ Lemma reducible_fill k e σ : reducible e σ → reducible (fill k e) σ.
 Proof.
   unfold reducible; simpl; rewrite /prim_step'; simpl.
   destruct 1 as [obs [e' [σ' [efs Hstep]]]].
-  case obs in Hstep; [|done]; case efs in Hstep; [|done].
-  inversion Hstep. simplify_eq. exists [], (fill (k ++ k0) e2'), σ', [].
-  apply (Ectx_prim_step _ _ _ _ (k ++ k0) e1' e2'); eauto.
+  case obs in Hstep; [|done].
+  inversion Hstep. simplify_eq. exists [], (fill (k ++ k0) e2'), σ', efs.
+  apply (Ectx_prim_step _ _ _ _ _ (k ++ k0) e1' e2'); eauto.
   by rewrite fill_app.
 Qed.
 
@@ -78,7 +76,6 @@ Proof.
   unfold irreducible; simpl. unfold prim_step'; simpl.
   intros obs ???.
   case obs; last auto. 
-  case efs; last auto.
   inversion 1.
   destruct k0 as [|f k0].
   - by simpl in H0; simplify_eq; inversion H2.
@@ -101,9 +98,8 @@ Proof.
   intros ??. unfold reducible; simpl; unfold prim_step'; simpl.
   intros [obs [e₂ [σ' [efs Hstep]]]].
   case obs in Hstep; [|done].
-  case efs in Hstep; [|done].
-  destruct (Ectxi_prim_step_inv _ _ _ _ _ H H0 Hstep) as [e' [Hstep' _]].
-  by exists [], e', σ', [].
+  destruct (Ectxi_prim_step_inv _ _ _ _ _ _ H H0 Hstep) as [e' [Hstep' _]].
+  by exists [], e', σ', efs.
 Qed.
 
 
@@ -116,34 +112,34 @@ Qed.
 (* [pure_prim_step] is the pure-step reduction relation:
    the relation [pure_prim_step e1 e2] holds if [e1] reduces to [e2]
    deterministically and without updating the state. *)
-Record pure_prim_step (e1 e2 : expr) := {
+Record pure_prim_step (e1 e2 : expr) efs := {
   pure_prim_step_safe σ :
-    prim_step e1 σ e2 σ;
-  pure_prim_step_det σ1 e2' σ2 :
-    prim_step e1 σ1 e2' σ2 → σ2 = σ1 ∧ e2' = e2
+    prim_step e1 σ e2 σ efs;
+  pure_prim_step_det σ1 e2' σ2 efs' :
+    prim_step e1 σ1 e2' σ2 efs' → σ2 = σ1 ∧ e2' = e2 ∧ efs = efs'
 }.
 
 
 (* -------------------------------------------------------------------------- *)
 (** Properties of [pure_prim_step]. *)
 
-Lemma pure_prim_step_imp_reducible e1 e2 :
-  pure_prim_step e1 e2 → (∀ σ, reducible e1 σ).
-Proof. intros Hstep ?. exists [], e2, σ, []. by apply Hstep. Qed.
+Lemma pure_prim_step_imp_reducible e1 e2 efs:
+  pure_prim_step e1 e2 efs → (∀ σ, reducible e1 σ).
+Proof. intros Hstep ?. exists [], e2, σ, efs. by apply Hstep. Qed.
 
-Lemma pure_prim_stepI e1 e2 :
-  (∀ σ, head_step e1 σ e2 σ) →
-    (∀ σ1 e2' σ2, prim_step e1 σ1 e2' σ2 → σ2 = σ1 ∧ e2' = e2) →
-      pure_prim_step e1 e2.
+Lemma pure_prim_stepI e1 e2 efs :
+  (∀ σ, head_step e1 σ e2 σ efs) →
+    (∀ σ1 e2' σ2 efs', prim_step e1 σ1 e2' σ2 efs' → σ2 = σ1 ∧ e2' = e2 ∧ efs = efs') →
+      pure_prim_step e1 e2 efs.
 Proof.
   intros Hhead_step Hstep_det. constructor; auto.
-  intros ?. apply (Ectx_prim_step _ _ _ _ [] e1 e2); by eauto.
+  intros ?. apply (Ectx_prim_step _ _ _ _ _ [] e1 e2); by eauto.
 Qed.
 
-Lemma pure_prim_stepI' e1 e2 :
-  (∀ σ, head_step e1 σ e2 σ) →
+Lemma pure_prim_stepI' e1 e2 efs :
+  (∀ σ, head_step e1 σ e2 σ efs) →
     (∀ k e1', e1 = fill k e1' → k = [] ∨ ∃ v, e1' = Val v) →
-      pure_prim_step e1 e2.
+      pure_prim_step e1 e2 efs.
 Proof.
   intros Hstep Hfill. apply pure_prim_stepI; auto.
   intros ???. inversion 1. simplify_eq.
@@ -151,35 +147,35 @@ Proof.
   specialize (Hstep σ1) as H3.
   inversion H2; simplify_eq; try naive_solver;
   inversion H3; simplify_eq; try naive_solver.
-  - unfold heap_upd in H9. simpl in H9.
-    rewrite lookup_insert in H9. done.
+  - unfold heap_upd in H10. simpl in H10.
+    rewrite lookup_insert in H10. done.
   - unfold heap_upd in H4. simpl in H4.
     rewrite lookup_insert in H4. done.
   - split; [|done]. destruct σ1 as [σ1].
     by rewrite /heap_upd /= insert_insert.
-  - unfold heap_upd in H10. simpl in H10.
-    rewrite lookup_insert in H10. done.
+  - unfold heap_upd in H11. simpl in H11.
+    rewrite lookup_insert in H11. done.
 Qed.
 
-Lemma val_not_pure v e : ¬ pure_prim_step (Val v) e.
+Lemma val_not_pure v e efs : ¬ pure_prim_step (Val v) e efs.
 Proof.
   intros Hstep.
-  specialize (pure_prim_step_imp_reducible _ _ Hstep {|heap:=∅|}) as H.
+  specialize (pure_prim_step_imp_reducible _ _ _ Hstep {|heap:=∅|}) as H.
   specialize (reducible_not_val (Val v) {|heap:=∅|} H); done.
 Qed.
 
-Lemma val_not_pure' v e e' : to_val e = Some v → ¬ pure_prim_step e e'.
+Lemma val_not_pure' v e e' efs : to_val e = Some v → ¬ pure_prim_step e e' efs.
 Proof. intro H1; rewrite <- (of_to_val _ _ H1). by apply val_not_pure. Qed.
 
-Lemma eff_not_pure m v k e : ¬ pure_prim_step (Eff m v k) e.
+Lemma eff_not_pure m v k e efs : ¬ pure_prim_step (Eff m v k) e efs.
 Proof.
   intros H0.
-  specialize (pure_prim_step_imp_reducible _ _ H0 {|heap:=∅|}).
+  specialize (pure_prim_step_imp_reducible _ _ _ H0 {|heap:=∅|}).
   specialize (eff_irreducible m v k {|heap:=∅|}).
   by rewrite <-not_reducible.
 Qed.
 
-Lemma eff_not_pure' p e e' : to_eff e = Some p → ¬ pure_prim_step e e'.
+Lemma eff_not_pure' p e e' efs : to_eff e = Some p → ¬ pure_prim_step e e' efs.
 Proof.
   intro H1. destruct p as ((m, v), k).
   rewrite <- (of_to_eff _ _ _ _ H1).
@@ -188,7 +184,7 @@ Qed.
 
 Lemma pure_prim_step_UnOp op v v' :
   un_op_eval op v = Some v' →
-    pure_prim_step (UnOp op (Val v)) (Val v').
+    pure_prim_step (UnOp op (Val v)) (Val v') [].
 Proof.
   intro Heval. apply pure_prim_stepI'; [intros ?; by apply UnOpS|].
   intros ??. destruct k as [|f k]; try destruct f; try naive_solver.
@@ -197,7 +193,7 @@ Qed.
 
 Lemma pure_prim_step_BinOp op v1 v2 v' :
   bin_op_eval op v1 v2 = Some v' →
-    pure_prim_step (BinOp op (Val v1) (Val v2)) (Val v').
+    pure_prim_step (BinOp op (Val v1) (Val v2)) (Val v') [].
 Proof.
   intro Heval. apply pure_prim_stepI'; [intros ?; by apply BinOpS|].
   intros ??. destruct k as [|f k]; try destruct f; try naive_solver.
@@ -207,7 +203,7 @@ Qed.
 
 Lemma pure_prim_step_beta f x e v :
   pure_prim_step ((App (Val $ RecV f x e) (Val v)))
-                 (subst' x v (subst' f (RecV f x e) e)).
+                 (subst' x v (subst' f (RecV f x e) e)) [].
 Proof.
   apply pure_prim_stepI'; [intros ?; by apply BetaS|].
   intros ??. destruct k as [|f' k]; [intros _; by left|].
@@ -220,14 +216,14 @@ Proof.
 Qed.
 
 Lemma pure_prim_step_Rec f x e :
-  pure_prim_step (Rec f x e) (Val $ RecV f x e).
+  pure_prim_step (Rec f x e) (Val $ RecV f x e) [].
 Proof.
   apply pure_prim_stepI'; [intros ?; by apply RecS|].
   intros ??. destruct k as [|f' k]; try destruct f'; by naive_solver.
 Qed.
 
 Lemma pure_prim_step_InjL v :
-  pure_prim_step (InjL $ Val v) (Val $ InjLV v).
+  pure_prim_step (InjL $ Val v) (Val $ InjLV v) [].
 Proof.
   apply pure_prim_stepI'; [intros ?; by apply InjLS|].
   intros ??. destruct k as [|f k]; try destruct f; try naive_solver.
@@ -235,7 +231,7 @@ Proof.
 Qed.
 
 Lemma pure_prim_step_InjR v :
-  pure_prim_step (InjR $ Val v) (Val $ InjRV v).
+  pure_prim_step (InjR $ Val v) (Val $ InjRV v) [].
 Proof.
   apply pure_prim_stepI'; [intros ?; by apply InjRS|].
   intros ??. destruct k as [|f k]; try destruct f; try naive_solver.
@@ -243,7 +239,7 @@ Proof.
 Qed.
 
 Lemma pure_prim_step_Case_InjL v e1 e2 :
-  pure_prim_step (Case (Val $ InjLV v) e1 e2) (App e1 (Val v)).
+  pure_prim_step (Case (Val $ InjLV v) e1 e2) (App e1 (Val v)) [].
 Proof.
   apply pure_prim_stepI'; [intros ?; by apply CaseLS|].
   intros ??. destruct k as [|f k]; try destruct f; try naive_solver.
@@ -251,7 +247,7 @@ Proof.
 Qed.
 
 Lemma pure_prim_step_Case_InjR v e1 e2 :
-  pure_prim_step (Case (Val $ InjRV v) e1 e2) (App e2 (Val v)).
+  pure_prim_step (Case (Val $ InjRV v) e1 e2) (App e2 (Val v)) [].
 Proof.
   apply pure_prim_stepI'; [intros ?; by apply CaseRS|].
   intros ??. destruct k as [|f k]; try destruct f; try naive_solver.
@@ -259,7 +255,7 @@ Proof.
 Qed.
 
 Lemma pure_prim_step_If e1 e2 b :
-  pure_prim_step (If (Val $ LitV $ LitBool b) e1 e2) (if b then e1 else e2).
+  pure_prim_step (If (Val $ LitV $ LitBool b) e1 e2) (if b then e1 else e2) [].
 Proof.
   apply pure_prim_stepI'; [
   intros ?; case b; [by apply IfTrueS|by apply IfFalseS]|].
@@ -268,15 +264,15 @@ Proof.
 Qed.
 
 Lemma pure_prim_step_If_true e1 e2 :
-  pure_prim_step (If (Val $ LitV $ LitBool true) e1 e2) e1.
+  pure_prim_step (If (Val $ LitV $ LitBool true) e1 e2) e1 [].
 Proof. by apply pure_prim_step_If. Qed.
 
 Lemma pure_prim_step_If_false e1 e2 :
-  pure_prim_step (If (Val $ LitV $ LitBool false) e1 e2) e2.
+  pure_prim_step (If (Val $ LitV $ LitBool false) e1 e2) e2 [].
 Proof. by apply pure_prim_step_If. Qed.
 
 Lemma pure_prim_step_Pair v1 v2 :
-  pure_prim_step (Pair (Val v1) (Val v2)) (Val $ PairV v1 v2).
+  pure_prim_step (Pair (Val v1) (Val v2)) (Val $ PairV v1 v2) [].
 Proof.
   apply pure_prim_stepI'; [intros ?; by apply PairS|].
   intros ??. destruct k as [|f k]; try destruct f; try naive_solver.
@@ -285,7 +281,7 @@ Proof.
 Qed.
 
 Lemma pure_prim_step_Fst v1 v2 :
-  pure_prim_step (Fst (Val $ PairV v1 v2)) (Val v1).
+  pure_prim_step (Fst (Val $ PairV v1 v2)) (Val v1) [].
 Proof.
   apply pure_prim_stepI'; [intros ?; by apply FstS|].
   intros ??. destruct k as [|f k]; try destruct f; try naive_solver.
@@ -293,15 +289,22 @@ Proof.
 Qed.
 
 Lemma pure_prim_step_Snd v1 v2 :
-  pure_prim_step (Snd (Val $ PairV v1 v2)) (Val v2).
+  pure_prim_step (Snd (Val $ PairV v1 v2)) (Val v2) [].
 Proof.
   apply pure_prim_stepI'; [intros ?; by apply SndS|].
   intros ??. destruct k as [|f k]; try destruct f; try naive_solver.
   intros [=]; destruct (fill_val' _ _ _ (eq_sym H0)) as [-> ->]; by eauto.
 Qed.
 
+Lemma pure_prim_step_Fork e :
+  pure_prim_step (Fork e) (Val $ LitV LitUnit) [e].
+Proof.
+  apply pure_prim_stepI'; [intros ?; by apply ForkS|].
+  intros ??. destruct k as [|f k]; try destruct f; try naive_solver.
+Qed.
+
 Lemma pure_prim_step_TryWithVal v h r :
-  pure_prim_step (TryWith (Val v) h r) (App r (Val v)).
+  pure_prim_step (TryWith (Val v) h r) (App r (Val v)) [].
 Proof.
   apply pure_prim_stepI'; [intros ?; by apply TryWithRetS|].
   intros ??. destruct k as [|f k]; try destruct f; try naive_solver.
@@ -310,7 +313,7 @@ Qed.
 
 Lemma pure_prim_step_TryWithMSEff v k h r :
   pure_prim_step (TryWith (Eff MS v k) h r)
-                 (App (App h (Val v)) (Val $ KontV k)).
+                 (App (App h (Val v)) (Val $ KontV k)) [].
 Proof.
   apply pure_prim_stepI.
   - intros ?. by apply TryWithMSEffS.
@@ -322,7 +325,7 @@ Proof.
 Qed.
 
 Lemma pure_prim_step_Kont k w :
-  pure_prim_step (App (Val $ KontV k) (Val w)) (fill k (Val w)).
+  pure_prim_step (App (Val $ KontV k) (Val w)) (fill k (Val w)) [].
 Proof.
   apply pure_prim_stepI'; [intros ?; by apply KontS|].
   intros ??. destruct k0 as [|f k0]; try destruct f; try naive_solver.
@@ -331,7 +334,7 @@ Proof.
 Qed.
 
 Lemma pure_prim_step_Do m v :
-  pure_prim_step (Do m (Val v)) (Eff m v []).
+  pure_prim_step (Do m (Val v)) (Eff m v []) [].
 Proof.
   apply pure_prim_stepI'; [intros ?; by apply DoS|].
   intros ??. destruct k as [|f k]; try destruct f; try naive_solver.
@@ -339,7 +342,7 @@ Proof.
 Qed.
 
 Lemma pure_prim_step_Eff `{NeutralFrame f} m v k :
-  pure_prim_step (fill_frame f (Eff m v k)) (Eff m v (f :: k)).
+  pure_prim_step (fill_frame f (Eff m v k)) (Eff m v (f :: k)) [].
 Proof.
   apply pure_prim_stepI; [intros ?; by apply H|].
   intros ??.
@@ -355,35 +358,37 @@ Proof.
     + destruct f, f1; simpl in H1; by naive_solver.
 Qed.
 
-Lemma pure_prim_step_fill_frame f e e' :
-  pure_prim_step e e' →
-    pure_prim_step (fill_frame f e) (fill_frame f e').
+Lemma pure_prim_step_fill_frame f e e' efs :
+  pure_prim_step e e' efs →
+    pure_prim_step (fill_frame f e) (fill_frame f e') efs.
 Proof.
   constructor.
   - intros ?. by apply (Ectxi_prim_step' f e e'), H.
-  - intros ??? Hstep.
+  - intros ???? Hstep.
     have not_val : to_val e = None.
     { by apply (reducible_not_val _ σ1),
-               (pure_prim_step_imp_reducible _ e'). }
+               (pure_prim_step_imp_reducible _ e' efs). }
     have not_eff : to_eff e = None.
     { by apply (reducible_not_eff _ σ1),
-               (pure_prim_step_imp_reducible _ e'). }
-    destruct (Ectxi_prim_step_inv f e _ _ _ not_val not_eff Hstep) as [e'' [He'' ->]].
-    by destruct (pure_prim_step_det _ _ H _ _ _ He'') as [-> ->].
+               (pure_prim_step_imp_reducible _ e' efs). }
+    destruct (Ectxi_prim_step_inv f e _ _ _ _ not_val not_eff Hstep) as [e'' [He'' ->]].
+    by destruct (pure_prim_step_det _ _ _ H _ _ _ _ He'') as (-> & -> & ->).
 Qed.
 
-Lemma pure_prim_step_fill k e e' :
-  pure_prim_step e e' →
-    pure_prim_step (fill k e) (fill k e').
+Lemma pure_prim_step_fill k e e' efs :
+  pure_prim_step e e' efs →
+    pure_prim_step (fill k e) (fill k e') efs.
 Proof.
   induction k as [|f k]; [done|].
   intros ?. simpl. apply pure_prim_step_fill_frame.
   apply IHk; eauto.
 Qed.
 
-Lemma tc_pure_prim_step_fill k e e' :
-  tc pure_prim_step e e' →
-    tc pure_prim_step (fill k e) (fill k e').
+Definition pure_prim_step_no_fork e e' := pure_prim_step e e' [].
+
+Lemma tc_pure_prim_step_no_fork_fill k e e' :
+  tc pure_prim_step_no_fork e e' →
+    tc pure_prim_step_no_fork (fill k e) (fill k e').
 Proof.
   induction 1.
   - apply tc_once.
@@ -392,34 +397,34 @@ Proof.
     by apply pure_prim_step_fill.
 Qed.
 
-Lemma rtc_pure_prim_step_fill k e e' :
-  rtc pure_prim_step e e' →
-    rtc pure_prim_step (fill k e) (fill k e').
+Lemma rtc_pure_prim_step_no_fork_fill k e e' :
+  rtc pure_prim_step_no_fork e e' →
+    rtc pure_prim_step_no_fork (fill k e) (fill k e').
 Proof.
   induction 1; [done|].
   apply (rtc_l _ _ (fill k y)); [|done].
   by apply pure_prim_step_fill.
 Qed.
 
-Lemma tc_pure_prim_step_fill_frame f e e' :
-  tc pure_prim_step e e' →
-    tc pure_prim_step (fill_frame f e) (fill_frame f e').
-Proof. by apply (tc_pure_prim_step_fill [f]). Qed.
+Lemma tc_pure_prim_step_no_fork_fill_frame f e e' :
+  tc pure_prim_step_no_fork e e' →
+    tc pure_prim_step_no_fork (fill_frame f e) (fill_frame f e').
+Proof. by apply (tc_pure_prim_step_no_fork_fill [f]). Qed.
 
-Lemma rtc_pure_prim_step_fill_frame f e e' :
-  rtc pure_prim_step e e' →
-    rtc pure_prim_step (fill_frame f e) (fill_frame f e').
-Proof. by apply (rtc_pure_prim_step_fill [f]). Qed.
+Lemma rtc_pure_prim_step_no_fork_fill_frame f e e' :
+  rtc pure_prim_step_no_fork e e' →
+    rtc pure_prim_step_no_fork (fill_frame f e) (fill_frame f e').
+Proof. by apply (rtc_pure_prim_step_no_fork_fill [f]). Qed.
 
-Lemma rtc_pure_prim_step_Eff `{NeutralEctx k} m v k' :
-  rtc pure_prim_step (fill k (Eff m v k')) (Eff m v (k ++ k')).
+Lemma rtc_pure_prim_step_no_fork_Eff `{NeutralEctx k} m v k' :
+  rtc pure_prim_step_no_fork (fill k (Eff m v k')) (Eff m v (k ++ k')).
 Proof.
   induction k as [|f k].
   - done.
   - specialize (ConsCtx_neutral_inv' _ _ H) as f_neutral.
     specialize (ConsCtx_neutral_inv  _ _ H) as  K_neutral.
     apply (rtc_r _ (fill_frame f (Eff m v (k ++ k')))); simpl.
-    + by apply rtc_pure_prim_step_fill_frame; auto.
+    + by apply rtc_pure_prim_step_no_fork_fill_frame; auto.
     + by apply pure_prim_step_Eff.
 Qed.
 
@@ -428,9 +433,9 @@ Qed.
 (** * Stateful Steps. *)
 
 (* Inversion principle for reduction of a one-shot continuation. *)
-Lemma prim_step_inv_Cont k l (w : val) σ e' σ' :
-  prim_step (App (Val $ (ContV k l)) (Val w)) σ e' σ' →
-    e' = fill k (Val w) ∧ σ' = heap_upd <[l := LitV $ LitBool $ true]> σ.
+Lemma prim_step_inv_Cont k l (w : val) σ e' σ' efs :
+  prim_step (App (Val $ (ContV k l)) (Val w)) σ e' σ' efs →
+    e' = fill k (Val w) ∧ σ' = heap_upd <[l := LitV $ LitBool $ true]> σ ∧ efs = [].
 Proof.
   intros Hstep. inversion Hstep.
   repeat ((destruct k0 as [|f k0]; [|destruct f; try naive_solver];
@@ -439,11 +444,12 @@ Qed.
 
 (* Inversion principle for the reification of evaluation
    context [k] as a one-shot continuation. *)
-Lemma prim_step_inv_TryWithOSEff (v : val) k h r σ e' σ' :
-  prim_step (TryWith (Eff OS v k) h r) σ e' σ' →
+Lemma prim_step_inv_TryWithOSEff (v : val) k h r σ e' σ' efs :
+  prim_step (TryWith (Eff OS v k) h r) σ e' σ' efs →
     ∃ l, σ.(heap) !! l = None ∧
          σ' = heap_upd <[l := LitV $ LitBool $ false]> σ ∧
-         e' = (App (App h (Val v)) (Val $ ContV k l)).
+         e' = (App (App h (Val v)) (Val $ ContV k l)) ∧
+         efs = [].
 Proof.
   intros Hstep. inversion Hstep.
   repeat ((destruct k0 as [|f k0]; [|destruct f; try naive_solver];
