theories/language/neutral_contexts.v
@@ -14,7 +14,7 @@ From language Require Import syntax semantics.
 
 Class NeutralFrame (f : frame) := {
   neutral_frame m v k σ :
-    head_step (fill_frame f (Eff m v k)) σ (Eff m v (f :: k)) σ
+    head_step (fill_frame f (Eff m v k)) σ (Eff m v (f :: k)) σ []
 }.
 Class NeutralEctx (k : ectx) := { neutral_ectx : Forall NeutralFrame k }.
 
@@ -33,46 +33,46 @@ Lemma ConsCtx_neutral_inv' f k : NeutralEctx (f :: k) → NeutralFrame f.
 Proof. inversion 1. by inversion neutral_ectx0. Qed.
 
 Instance AppLCtx_neutral v2 : NeutralFrame (AppLCtx v2).
-Proof. constructor => v k σ. by apply AppLEffS. Qed.
+Proof. constructor => m v k σ. by apply AppLEffS. Qed.
 Instance AppRCtx_neutral e1 : NeutralFrame (AppRCtx e1).
-Proof. constructor => v k σ. by apply AppREffS. Qed.
+Proof. constructor => m v k σ. by apply AppREffS. Qed.
 Instance DoCtx_neutral m : NeutralFrame (DoCtx m).
-Proof. constructor => v k σ. by apply DoEffS. Qed.
+Proof. constructor => m' v k σ. by apply DoEffS. Qed.
 Instance UnOpCtx_neutral op : NeutralFrame (UnOpCtx op).
-Proof. constructor => v k σ. by apply UnOpEffS. Qed.
+Proof. constructor => m v k σ. by apply UnOpEffS. Qed.
 Instance BinOpLCtx_neutral op v2 : NeutralFrame (BinOpLCtx op v2).
-Proof. constructor => v k σ. by apply BinOpLEffS. Qed.
+Proof. constructor => m v k σ. by apply BinOpLEffS. Qed.
 Instance BinOpRCtx_neutral op e1 : NeutralFrame (BinOpRCtx op e1).
-Proof. constructor => v k σ. by apply BinOpREffS. Qed.
+Proof. constructor => m v k σ. by apply BinOpREffS. Qed.
 Instance IfCtx_neutral e1 e2 : NeutralFrame (IfCtx e1 e2).
-Proof. constructor => v k σ. by apply IfEffS. Qed.
+Proof. constructor => m v k σ. by apply IfEffS. Qed.
 Instance PairLCtx_neutral v2 : NeutralFrame (PairLCtx v2).
-Proof. constructor => v k σ. by apply PairLEffS. Qed.
+Proof. constructor => m v k σ. by apply PairLEffS. Qed.
 Instance PairRCtx_neutral e1 : NeutralFrame (PairRCtx e1).
-Proof. constructor => v k σ. by apply PairREffS. Qed.
+Proof. constructor => m v k σ. by apply PairREffS. Qed.
 Instance FstCtx_neutral : NeutralFrame FstCtx.
-Proof. constructor => v k σ. by apply FstEffS. Qed.
+Proof. constructor => m v k σ. by apply FstEffS. Qed.
 Instance SndCtx_neutral : NeutralFrame SndCtx.
-Proof. constructor => v k σ. by apply SndEffS. Qed.
+Proof. constructor => m v k σ. by apply SndEffS. Qed.
 Instance InjLCtx_neutral : NeutralFrame InjLCtx.
-Proof. constructor => v k σ. by apply InjLEffS. Qed.
+Proof. constructor => m v k σ. by apply InjLEffS. Qed.
 Instance InjRCtx_neutral : NeutralFrame InjRCtx.
-Proof. constructor => v k σ. by apply InjREffS. Qed.
+Proof. constructor => m v k σ. by apply InjREffS. Qed.
 Instance CaseCtx_neutral e1 e2 : NeutralFrame (CaseCtx e1 e2).
-Proof. constructor => v k σ. by apply CaseEffS. Qed.
+Proof. constructor => m v k σ. by apply CaseEffS. Qed.
 Instance AllocCtx_neutral : NeutralFrame AllocCtx.
-Proof. constructor => v k σ. by apply AllocEffS. Qed.
+Proof. constructor => m v k σ. by apply AllocEffS. Qed.
 Instance LoadCtx_neutral : NeutralFrame LoadCtx.
-Proof. constructor => v k σ. by apply LoadEffS. Qed.
+Proof. constructor => m v k σ. by apply LoadEffS. Qed.
 Instance StoreLCtx_neutral v2 : NeutralFrame (StoreLCtx v2).
-Proof. constructor => v k σ. by apply StoreLEffS. Qed.
+Proof. constructor => m v k σ. by apply StoreLEffS. Qed.
 Instance StoreRCtx_neutral e1 : NeutralFrame (StoreRCtx e1).
-Proof. constructor => v k σ. by apply StoreREffS. Qed.
+Proof. constructor => m v k σ. by apply StoreREffS. Qed.
 
 Lemma TryWithCtx_not_neutral e2 e3 : ¬ NeutralFrame (TryWithCtx e2 e3).
 Proof.
   intros ?. cut (head_step
     (TryWith (Eff MS (LitV LitUnit) []) e2 e3) {|heap:=∅|}
-    (Eff MS (LitV LitUnit) [TryWithCtx e2 e3]) {|heap:=∅|});
+    (Eff MS (LitV LitUnit) [TryWithCtx e2 e3]) {|heap:=∅|} []);
   [inversion 1|apply H]; done.
 Qed.
